abp/Medium/medUnfairAut.thy
@@ -71,21 +71,152 @@ lemma medunfair_step_msg [simp]: "spsConcIn (mediumIn_i (Msg m)) medUnfair
   by (metis medState.exhaust)
 
 
-lemma sps2spf_step_single: assumes "spsConcIn input sps = spsConcOut output sps2"
-          and "spf \<in> uspecSet sps"
-        obtains spf2 where "spfConcIn input\<cdot>spf = spfConcOut output\<cdot>spf2" and "spf2 \<in> uspecSet sps2"
-  oops
+
+
+
+(* Allgemein det-step*)
+lemma uspecimage_rep_eq: assumes "\<And>x y. ((ufclDom\<cdot>x = ufclDom\<cdot>y \<and> ufclRan\<cdot>x = ufclRan\<cdot>y) \<Longrightarrow>
+    (ufclDom\<cdot>(f x) = ufclDom\<cdot>(f y) \<and> ufclRan\<cdot>(f x) = ufclRan\<cdot>(f y)))" 
+  shows "Rep_uspec (uspecImage f S) =((setrevImage f (uspecRevSet\<cdot>S)),
+    Discr (ufclDom\<cdot> (f (ufunclLeast (uspecDom\<cdot> S) (uspecRan\<cdot> S)))),
+    Discr (ufclRan\<cdot> (f (ufunclLeast (uspecDom\<cdot> S) (uspecRan\<cdot> S)))))"
+  by (simp add: assms setrevImage_def ufuncldom_least_dom ufuncldom_least_ran uspecImage_def uspec_allDom uspec_allRan)
+
+lemma uspecimage_set: assumes "\<And>x y. ((ufclDom\<cdot>x = ufclDom\<cdot>y \<and> ufclRan\<cdot>x = ufclRan\<cdot>y) \<Longrightarrow>
+    (ufclDom\<cdot>(f x) = ufclDom\<cdot>(f y) \<and> ufclRan\<cdot>(f x) = ufclRan\<cdot>(f y)))" 
+  shows "uspecSet (uspecImage f sps) = f ` (uspecSet sps)"
+  apply(simp add: uspecSet_def uspecRevSet_def)
+  apply(subst uspecimage_rep_eq)
+  using assms apply blast
+  by (simp add: rep_rev_revset setrevImage_def)
+
+lemma spsconcin_set:  "uspecSet (spsConcIn In sps) = (Rep_cfun (spfConcIn In)) ` (uspecSet sps)"
+  apply(simp add: spsConcIn_def)
+  apply(rule uspecimage_set)
+  by (simp add: spfconcin_uspec_iamge_well ufclRan_ufun_def)
+
+lemma spsconcout_set:  "uspecSet (spsConcOut Out sps) = (Rep_cfun (spfConcOut Out)) ` (uspecSet sps)"
+  apply(simp add: spsConcOut_def)
+  apply(rule uspecimage_set)
+  by (simp add: ufclDom_ufun_def ufclRan_ufun_def)
+
+lemma spsonestep_spf: assumes "spsConcIn In sps1 = spsConcOut Out sps2" 
+  shows "(Rep_cfun (spfConcIn In)) `(uspecSet sps1) = (Rep_cfun (spfConcOut Out)) ` uspecSet sps2"
+  by (metis assms spsconcin_set spsconcout_set)
+
+lemma spsonestep_spf_exists: assumes "spsConcIn In sps1 = spsConcOut Out sps2" and "spf1 \<in> uspecSet sps1"
+  shows  "\<exists>spf2. spf2 \<in> uspecSet sps2 \<and> spfConcIn In\<cdot>spf1 = spfConcOut Out\<cdot>spf2"
+  by (metis (no_types, hide_lams) assms(1) assms(2) image_iff spsconcin_set spsconcout_set)
+  
+
+
+
+(* Global, non-det-step *)
+
+lemma uspecflatten_rep_eq: "Rep_rev_uspec (uspecFlatten Dom Ran uspec) 
+  = ((setflat\<cdot>(Rep_rev_uspec ` (inv Rev (uspec_set_filter Dom Ran\<cdot>uspec)))))"
+  apply(simp add: uspecFlatten_def)
+  using rep_abs_rev_simp uspecflatten_well by blast
+
+lemma uspecflatten_set: "uspecSet (uspecFlatten Dom Ran (Rev uspecs)) = 
+    (Set.filter (\<lambda> uf. ufDom\<cdot>uf = Dom \<and> ufRan\<cdot>uf = Ran) (\<Union> (uspecSet ` uspecs)))"
+  apply(simp add: uspecSet_def uspecRevSet_def)
+  apply(simp add: uspecflatten_rep_eq)
+  apply(simp add: setflat_union uspec_set_filter_def setrevFilter_def)
+  apply auto
+  apply blast
+  apply (metis ufclDom_ufun_def uspec_allDom uspecrevset_insert)
+  apply (metis rep_rev_revset ufclDom_ufun_def uspec_allDom)
+  apply (metis rep_rev_revset ufclRan_ufun_def uspec_allRan)
+  apply (metis ufclRan_ufun_def uspec_allRan uspecrevset_insert)
+  by (metis (mono_tags, lifting) member_filter rep_rev_revset ufclDom_ufun_def ufclRan_ufun_def uspec_allDom uspec_allRan)
+
+lemma ndaconcoutflat_set: 
+  "uspecSet (ndaConcOutFlatten Dom Ran (Rev Transition) h) = 
+    (Set.filter (\<lambda> uf. ufDom\<cdot>uf = Dom \<and> ufRan\<cdot>uf = Ran) (\<Union> (((\<lambda> (s, sb). uspecSet (ndaTodo_h Dom Ran sb (h s))) ` Transition))))"
+  apply(simp add: ndaConcOutFlatten_def setrevImage_def)
+  apply(simp add: uspecflatten_set)
+  by (simp add: case_prod_beta')
+
+lemma ndaconcout_subset: assumes "(nextState, Out) \<in> Transition" and "uspecDom\<cdot>(h nextState) = Dom" and "uspecRan\<cdot>(h nextState) = Ran"
+  shows " uspecSet(ndaTodo_h Dom Ran Out (h nextState)) \<subseteq> uspecSet (ndaConcOutFlatten Dom Ran (Rev Transition) h) "
+  apply(subst ndaconcoutflat_set)
+  apply rule
+  by (smt UN_iff assms(1) assms(2) assms(3) case_prod_beta' fst_conv member_filter ndaconcoutflat_set ndaconout_one snd_conv)
+
+
+lemma ndaconcout_get: assumes "spf \<in> uspecSet (ndaConcOutFlatten Dom Ran Transition h)"
+  shows "\<exists> nextState Out. (nextState, Out) \<in> (inv Rev) Transition 
+          \<and>spf \<in> uspecSet(ndaTodo_h Dom Ran Out (h nextState))"
+  by (metis (mono_tags, lifting) UN_iff assms case_prod_beta' member_filter ndaconcoutflat_set prod.collapse rev_inv_rev)
+
+lemma ndastep_spf: assumes "spsConcIn In sps = ndaConcOutFlatten Dom Ran (Rev Transition) h" and "spf\<in>uspecSet sps"
+  and "\<And>nextState Out. (nextState, Out) \<in> Transition \<Longrightarrow> ubLen (ubRestrict Ran\<cdot>(ubUp\<cdot>Out)) < \<infinity>"
+  shows "\<exists> nextState Out spf2. (nextState, Out) \<in> Transition 
+          \<and> spf2 \<in>(uspecSet (h nextState))
+          \<and> spfConcIn In\<cdot>spf = spfConcOut Out\<cdot>spf2"
+proof - 
+  have "spfConcIn In\<cdot>spf \<in> uspecSet (ndaConcOutFlatten Dom Ran (Rev Transition) h)"
+    by (metis assms(1) assms(2) rev_image_eqI spsconcin_set)
+  from this obtain nextState Out where  in_trans: "(nextState, Out) \<in> Transition" 
+      and step_h:"spfConcIn In\<cdot>spf \<in> uspecSet(ndaTodo_h Dom Ran Out (h nextState))"
+    using ndaconcout_get by force
+  hence "ubLen (ubRestrict Ran\<cdot>(ubUp\<cdot>Out)) < \<infinity>"
+    using assms(3) by blast
+  hence "spfConcIn In\<cdot>spf \<in> uspecSet(spsConcOut Out (h nextState))" using step_h ndaTodo_h_def by metis
+  thus ?thesis
+    using in_trans spsconcout_set by fastforce
+qed
+
+lemma ndaconcout_get_step: assumes "spf \<in> uspecSet (ndaConcOutFlatten Dom Ran Transition h)"
+  shows "\<exists> nextState Out. (nextState, Out) \<in> (inv Rev) Transition 
+          \<and>spf \<in> uspecSet(ndaTodo_h Dom Ran Out (h nextState))"
+  by (metis (mono_tags, lifting) UN_iff assms case_prod_beta' member_filter ndaconcoutflat_set prod.collapse rev_inv_rev)
+
+
+lemma lnat_1_inf [simp]: "1 < \<infinity>"
+  unfolding one_lnat_def
+  by simp
+
+
+
+(* Medium-spezifisch *)
+
+lemma medtodo [simp]: "ndaTodo_h mediumDom mediumRan (mediumOut_o m) sps = spsConcOut (mediumOut_o m) sps"
+  by(auto simp add: ndaTodo_h_def)
 
 lemma medunfair_spf_step_tick [simp]: assumes "spf \<in> uspecSet (medUnfair)"
-  shows "spfConcIn (mediumIn_i -)\<cdot>spf = spfConcOut (mediumOut_o -)\<cdot>spf"
-  oops
+  obtains spf2 where "spf2\<in>uspecSet medUnfair" and "spfConcIn (mediumIn_i -)\<cdot>spf = spfConcOut (mediumOut_o -)\<cdot>spf2"
+  using assms medunfair_step_tick spsonestep_spf_exists by blast
+
+lemma med_msg_step_h: assumes "spf\<in>uspecSet medUnfair"
+  shows "\<exists> nextState Out spf2. (nextState, Out) \<in> ({(Single, mediumOut_o -), (Single, mediumOut_o (Msg m))}) 
+          \<and> spf2 \<in>(uspecSet medUnfair)
+          \<and> spfConcIn (mediumIn_i (Msg m))\<cdot>spf = spfConcOut Out\<cdot>spf2"
+  by(rule ndastep_spf [of "(mediumIn_i (Msg m))" medUnfair], auto simp add: assms)
+
+lemma medunfair_spf_step_msg [simp]: assumes "spf \<in> uspecSet (medUnfair)"
+  shows "\<exists> out spf2. spf2\<in>uspecSet medUnfair \<and> spfConcIn (mediumIn_i (Msg m))\<cdot>spf = spfConcOut (mediumOut_o out)\<cdot>spf2 \<and> out\<in>{-, Msg m}"
+  using assms med_msg_step_h by fastforce
+
+
+
+(* Autogenerate: *)
+lemma med_spf_strict[simp]: "spf\<in>uspecSet (medUnfair) \<Longrightarrow> (spf \<rightleftharpoons> ubLeast mediumDom) = ubLeast mediumRan"
+  sorry
+
+lemma med_spf_strict2[simp]: "spf\<in>uspecSet (medUnfair) \<Longrightarrow> (spf \<rightleftharpoons> (mediumIn_stream_i\<cdot>\<epsilon>)) = ubLeast mediumRan"
+  by (simp add: medin_stream_least)
 
 (* Final Proof *)
 lemma medunfair_dom [simp]: assumes "spf \<in> uspecSet medUnfair"
   shows "tsynDom\<cdot>(medium_get_stream_o\<cdot>(spf \<rightleftharpoons> mediumIn_stream_i\<cdot>s)) \<subseteq> tsynDom\<cdot>s"
   using assms apply(induction s arbitrary: spf rule:ind)
-  apply(rule admI)
-    apply auto
+    apply(rule adm_all, rule admI)
+    apply (rule, simp)
+    defer
+    apply (simp)
+  
   oops
 
 end
